PrefixSerializableDefinitions.v
@@ -1,0 +1,19 @@
+Require Import Coq.Strings.String.
+
+Set Implicit Arguments.
+
+Local Open Scope string_scope.
+
+Class Serializable A :=
+  { to_string : A -> string }.
+Class Deserializable A :=
+  { from_string : string -> option A * string }.
+
+Class PrefixSerializable A :=
+  { serialize :> Serializable A;
+    deserialize :> Deserializable A;
+    from_to_string : forall x, from_string (to_string x) = (Some x, "");
+    prefix_closed : forall s1 s2 x, fst (from_string s1) = Some x -> from_string (s1 ++ s2) = (Some x, snd (from_string s1) ++ s2) }.
+
+Arguments serialize _ !_ / .
+Arguments deserialize _ !_ / .
